improve extraction, prove that reqs get answered

extraction/lib/DynamicShim.ml
@@ -3,7 +3,7 @@ open Unix
 open Sys
 
 module M = Marshal
-               
+
 module type DYNAMIC_ARRANGEMENT = sig
   type name
   type state
@@ -17,30 +17,57 @@ module type DYNAMIC_ARRANGEMENT = sig
   val handleTick : name -> state -> res
   val handleTimeout : name -> name -> state -> res
   val setTick : name -> state -> float
+  val query_timeout : float
   val debug : bool
   val debugRecv : state -> (name * msg) -> unit
   val debugSend : state -> (name * msg) -> unit
   val debugTick : state -> unit
+  val debugTimeout : state -> (name * msg) -> unit
 end
-
 module Shim (A: DYNAMIC_ARRANGEMENT) = struct
+  (* assoc list of start times mapping to (name, msg) pairs *)
+
+  type requests = (float * A.name * A.msg) list
+
+  let empty_requests = []
+
+  let rec timed_out_requests timeout ts : (A.name * A.msg) list =
+    let now = Unix.gettimeofday () in
+    match ts with
+    | (t, dst, msg) :: rest ->
+       if now -. t > timeout
+       then (dst, msg) :: timed_out_requests timeout rest
+       else timed_out_requests timeout rest
+    | [] -> []
+
+  let rec record_request rs (dst, msg) : requests =
+    if A.is_request msg
+    then (Unix.gettimeofday (), dst, msg) :: rs
+    else rs
+
+  let remove_requests rs dst : requests =
+    List.filter (fun (_, d, _) -> d == dst) rs
 
   type env =
     {
-      usock : file_descr
+      usock : file_descr;
+      mutable open_requests : requests;
+      mutable last_tick : float
     }
 
   let setup nm =
     Random.self_init ();
     let port = snd (A.addr_of_name nm) in
     let env =
-      { usock = socket PF_INET SOCK_DGRAM 0
+      { usock = socket PF_INET SOCK_DGRAM 0;
+        open_requests = empty_requests;
+        last_tick = Unix.gettimeofday ()
       }
     in
     setsockopt env.usock SO_REUSEADDR true;
     bind env.usock (ADDR_INET (inet_addr_any, port));
     env
-    
+
   let sendto sock buf addr =
     ignore (Unix.sendto sock buf 0 (String.length buf) [] addr)
 
@@ -50,14 +77,18 @@ module Shim (A: DYNAMIC_ARRANGEMENT) = struct
 
   let respond_to_client sock r =
     ignore (Unix.send sock (r ^ "\n") 0 (String.length r) [])
-                   
+
   let unpack_msg buf : A.msg =
     M.from_string buf 0
 
+  let respond_one env s p =
+    (if A.debug then A.debugSend s p);
+    env.open_requests <- record_request env.open_requests p;
+    send env p
+
   let respond env (s, ps) =
-    List.iter (fun p -> (if A.debug then A.debugSend s p); send env p) ps;
-    s
-    
+    List.iter (respond_one env s) ps; s
+
   let recv_step env nm s =
     let len = 4096 in
     let buf = String.make len '\x00' in
@@ -67,13 +98,36 @@ module Shim (A: DYNAMIC_ARRANGEMENT) = struct
      | ADDR_UNIX _ -> failwith "UNEXPECTED MESSAGE FROM UNIX ADDR"
      | ADDR_INET (addr,port) -> A.name_of_addr (string_of_inet_addr addr, port)) in
     let m = unpack_msg buf in
-    let s' = respond env (A.handleNet nm src m s) in
-    (if A.debug then A.debugRecv s' (src, m)); s'
+    let s' = respond env (A.handleNet src nm m s) in
+    (if A.debug then A.debugRecv s' (src, m));
+    env.open_requests <- remove_requests env.open_requests src;
+    print_int (List.length env.open_requests);
+    s'
 
   let tick_step env nm s =
     (if A.debug then A.debugTick s);
+    env.last_tick <- Unix.gettimeofday ();
     let x = A.handleTick nm s in
     respond env x
+
+  let do_timeout env nm (s, sends) (dst, msg) =
+    let (s', sends') = A.handleTimeout nm dst s in
+    env.open_requests <- remove_requests env.open_requests dst;
+    print_int (List.length env.open_requests);
+    A.debugTimeout s (dst, msg);
+    (s', sends @ sends')
+
+  let timeout_step env nm s =
+    let timeouts = timed_out_requests A.query_timeout env.open_requests in
+    let res = List.fold_left (do_timeout env nm) (s, []) timeouts in
+    print_int (List.length env.open_requests);
+    respond env res
+
+  let maybe_tick env nm s =
+    print_float ((Unix.gettimeofday ()) -. env.last_tick);
+    if (Unix.gettimeofday ()) -. env.last_tick > A.setTick nm s
+    then tick_step env nm s
+    else (print_string "not long enough yet\n"; s)
 
   let rec my_select rs ws es t =
     try select rs ws es t
@@ -82,18 +136,19 @@ module Shim (A: DYNAMIC_ARRANGEMENT) = struct
 
   let rec eloop env nm s =
     let (fds, _, _) = my_select [env.usock] [] [] (A.setTick nm s) in
-    let s' =
-      match List.mem env.usock fds with
-      | true -> (try (recv_step env nm s) with
-                 | _ -> s)
-      | _ -> tick_step env nm s in
-    eloop env nm s'
+    let s' = if List.mem env.usock fds
+             then (try (recv_step env nm s) with
+                   | _ -> s)
+             else s in
+    let s'' = timeout_step env nm s' in
+    let s''' = maybe_tick env nm s'' in
+    eloop env nm s'''
 
   let default v o =
     match o with
     | None -> v
     | Some v' -> v'
-  
+
   let main nm knowns =
     print_endline "running setup";
     let env = setup nm in
