systems/Chord.v
@@ -28,10 +28,11 @@ Inductive payload :=
 | Pong : payload.
 
 Definition client_payload msg := exists (p : pointer), msg = GetBestPredecessor p.
-Definition request_payload msg := (exists (p : pointer), msg = GetBestPredecessor p)
-                                                      \/ msg = GetSuccList
-                                                      \/ msg = GetPredAndSuccs
-                                                      \/ msg = Ping.
+Inductive request_payload : payload -> Prop :=
+| req_GetBestPredecessor : forall m p, m = GetBestPredecessor p -> request_payload m
+| req_GetSuccList : request_payload GetSuccList
+| req_GetPredAndSuccs : request_payload GetPredAndSuccs
+| req_Ping : request_payload Ping.
 
 Definition is_request (p : payload) :=
   match p with
@@ -238,7 +239,7 @@ Definition start_handler (h : addr) (knowns : list addr) : data * list (addr * p
       let p := make_pointer k in
       let succs := map make_pointer nowns in
       let st := Data (make_pointer h) (Some p) succs p true None None false in
-      start_query h st Stabilize
+      (st, [])
     (* garbage data, shouldn't happen *)
     | [] => (Data (make_pointer h) None [] (make_pointer h) false None None false, [])
   end.
@@ -276,3 +277,52 @@ Definition timeout_handler (src : addr) (dst : addr) (st : data) : data * list (
                        else (st, []) (* shouldn't happen *)
     | None => (st, []) (* shouldn't happen *)
  end.
+
+Lemma is_request_same_as_request_payload : forall msg : payload,
+    is_request msg = true <-> request_payload msg.
+Proof.
+  intuition.
+  - induction msg.
+    * constructor 1 with (p := p). reflexivity.
+    * inversion H.
+    * constructor.
+    * inversion H.
+    * constructor.
+    * inversion H.
+    * inversion H.
+    * constructor.
+    * inversion H.
+  - induction msg; intuition; inversion H; inversion H0.
+Qed.
+
+Lemma requests_are_always_responded_to : forall src dst msg st sends,
+    request_payload msg ->
+    (st, sends) = recv_handler src dst msg st ->
+    exists res, In (src, res) sends.
+Proof.
+  intuition.
+  induction msg.
+  * inversion H.
+    inversion H0.
+    exists (GotBestPredecessor (best_predecessor dst st (id_of p))).
+    intuition.
+  * inversion H.
+    inversion H1.
+  * inversion H0.
+    exists (GotSuccList (succ_list st)).
+    intuition.
+  * inversion H. 
+    inversion H1.
+  * inversion H0.
+    exists (GotPredAndSuccs (pred st) (succ_list st)).
+    intuition.
+  * inversion H.
+    inversion H1.
+  * inversion H.
+    inversion H1.
+  * inversion H0.
+    exists Pong.
+    intuition.
+  * inversion H.
+    inversion H1.
+Qed.
