extraction/chord/ml/ChordArrangement.ml
@@ -15,7 +15,7 @@ let show_addr a =
   string_of_int a
 
 let show_pointer p =
-  string_of_int (ExtractedChord.id_of p)
+  "(" ^ string_of_int (ExtractedChord.id_of p) ^ ", " ^ show_addr (ExtractedChord.addr_of p) ^ ")"
 
 let show_pointer_list ps =
   let strs = map show_pointer ps in
@@ -39,27 +39,42 @@ let show_msg = function
   | Ping -> "Ping"
   | Pong -> "Pong"
 
-let show_st_id st =
-  string_of_int (ExtractedChord.id_of (ExtractedChord.ptr st))
+let show_query = function
+  | Rectify p -> "Rectify " ^ show_pointer p
+  | Stabilize -> "Stabilize"
+  | Stabilize2 p -> "Stabilize2 " ^ show_pointer p
+  | Join p -> "Join " ^ show_pointer p
+  | Join2 p -> "Join2 " ^ show_pointer p
 
+let show_st_ptr st =
+  show_pointer (ExtractedChord.ptr st)
+let show_request (ptr, q) =
+  "query(" ^ show_pointer ptr ^ ", " ^ show_query q ^")"
+let show_st_cur_request st =
+  map_default show_request "None" (ExtractedChord.cur_request st)
 let show_st st = 
-  let prefix = "node(" ^ show_st_id st ^ "):" in
+  let prefix = "node(" ^ show_st_ptr st ^ "):" in
   let log msg = info (prefix ^ msg) in
   log ("succ_list := " ^ show_pointer_list (ExtractedChord.succ_list st));
-  log ("pred := " ^ show_opt_pointer (ExtractedChord.pred st))
+  log ("pred := " ^ show_opt_pointer (ExtractedChord.pred st));
+  log ("known := " ^ show_pointer (ExtractedChord.known st));
+  log ("joined := " ^ string_of_bool (ExtractedChord.joined st));
+  log ("rectify_with := " ^ show_opt_pointer (ExtractedChord.rectify_with st));
+  log ("cur_request := " ^ show_st_cur_request st);
+  log ("query_sent := " ^ string_of_bool (ExtractedChord.query_sent st))
 
 let log_recv src msg =
-  dbg ("recv at " ^ show_addr src ^ ": " ^ show_msg msg)
+  dbg ("recv from " ^ show_addr src ^ ": " ^ show_msg msg)
 
 let log_send dst msg =
-  dbg ("send from " ^ show_addr dst ^ ":" ^ show_msg msg)
+  dbg ("send to " ^ show_addr dst ^ ":" ^ show_msg msg)
 
 module ChordDebugArrangement = struct
   type name = ExtractedChord.addr
   type state = ExtractedChord.data
   type msg = ExtractedChord.payload
   type res = state * (name * msg) list
-  (* should I put these two fns in coq *)
+  (* should put these two in coq so i can prove (name_of_addr (addr_of_name n)) = n *)
   let addr_of_name n =
       ("127.0.0.1", n)
   let name_of_addr (s, p) =
@@ -69,10 +84,15 @@ module ChordDebugArrangement = struct
   let handleTick = ExtractedChord.tick_handler
   let handleTimeout = ExtractedChord.timeout_handler
   let setTick n s = 5.0
+  let query_timeout = 10.0
   let debug = true
   let debugInit n knowns = dbg "running init"
   let debugRecv st (src, msg) = show_st st; log_recv src msg
   let debugSend st (dst, msg) = show_st st; log_send dst msg
   let debugTick st = show_st st
+  let debugTimeout st (dead, msg) =
+    dbg ("request " ^ show_msg msg
+         ^ " from " ^ show_pointer (ptr st)
+         ^ " to " ^ show_addr dead ^ " timed out")
   let init = ExtractedChord.start_handler
 end
